common/InvariantAlgebra.v
@@ -1,0 +1,108 @@
+Require Import Coqlib.
+Require Export LanguageInterface.
+Require Export Smallstep.
+Require Import CallconvAlgebra Invariant.
+Require Import SmallstepLinkingSafe.
+
+(* Refinement of invariants *)
+
+(* [I1] is refined by [I2], meaning that any lts is safe under [I2] is
+also safe under [I1] *)
+Definition inv_ref {li} (I1 I2: invariant li) :=
+  forall w1 se q,
+    symtbl_inv I1 w1 se ->
+    query_inv I1 w1 q ->
+    exists w2,
+      symtbl_inv I2 w2 se
+      /\ query_inv I2 w2 q
+      /\ forall r,
+        reply_inv I2 w2 r ->
+        reply_inv I1 w1 r.
+
+Definition inveqv {li} (I1 I2: invariant li) :=
+  inv_ref I1 I2 /\ inv_ref I2 I1.
+
+Global Instance inv_ref_preo li:
+  PreOrder (@inv_ref li).
+Proof.
+  split.
+  - intros I w1 se q SINV QINV.
+    eauto.
+  - intros I1 I2 I3 R1 R2 w1 se q SINV QINV.
+    edestruct R1 as (w2' & SINV' & QINV' & RINV'); eauto.
+    edestruct R2 as (w3' & SINV'' & QINV'' & RINV''); eauto 10.
+Qed.
+
+Global Instance inveqv_equiv li:
+  Equivalence (@inveqv li).
+Proof.
+  split.
+  - intros I. split; reflexivity.
+  - intros I1 I2. unfold inveqv. tauto.
+  - intros I1 I2 I3 [R1 R1'] [R2 R2'].
+    split; etransitivity; eauto.
+Qed.
+
+Global Instance inv_ref_po li:
+  PartialOrder (@inveqv li) (@inv_ref li).
+Proof.
+  firstorder.
+Qed.
+
+Global Instance open_safety_inv_ref:
+  Monotonic
+    (@module_type_safe)
+    (forallr - @ liA, forallr - @ liB, inv_ref ++>
+     inv_ref --> 
+     forallr - @ L, forallr - @ PS,
+     impl
+    ).
+Proof.
+  intros liA liB IA1 IA2 RA IB1 IB2 RB L PS [SAFE].
+  red in RB. econstructor.
+  inv SAFE.
+  set (ms se wB2 s :=
+         exists wB1, msafek_invariant se wB1 s
+                /\ symtbl_inv IB1 wB1 se
+                /\ forall r, reply_inv IB1 wB1 r ->
+                       reply_inv IB2 wB2 r).  
+  eapply Module_ksafe_components with (msafek_invariant := ms).
+  intros se wB2 SINV2 VSE.
+  econstructor.
+  - intros s t s' (wB1 & INV & SINV1 & RINV) STEP.
+    exists wB1. repeat apply conj; auto.
+    eapply internal_step_preserves; eauto.
+  - intros s (wB1 & INV & SINV1 & RINV).
+    eapply internal_state_progress; eauto.
+  - intros q VQ QINV2.
+    edestruct RB as (wB1 & SINV1 & QINV1 & RINV); eauto.
+    edestruct @initial_preserves_progress as (s & INIT & INIT1); eauto.
+    exists s. split; auto.
+    intros s' INIT'.
+    exists wB1. repeat apply conj; auto.
+  - intros s q (wB1 & INV & SINV1 & RINV) ATEXT.
+    edestruct @external_preserves_progress as (wA1 & SINV1' & QINV1 & RINV1); eauto.
+    edestruct RA as (wA2 & SINV2' & QINV2' & RINV'); eauto.
+    exists wA2. repeat apply conj; auto.
+    intros r RINV2. specialize (RINV' r RINV2).
+    edestruct RINV1 as (s' & AFEXT & AFEXT'); eauto.
+    exists s'. split; auto.
+    intros. exists wB1.
+    repeat apply conj; auto.
+  - intros s r (wB1 & SINV1 & QINV1 & RINV) FINAL.
+    eapply RINV. eapply final_state_preserves; eauto.
+Qed.
+
+Lemma test_rewrite_inv_ref_fail {liA liB} : forall (IA: invariant liA) (IB1 IB2: invariant liB) L PS,
+    inv_ref IB2 IB1 ->
+    module_type_safe IA IB1 L PS ->
+    module_type_safe IA IB2 L PS.
+Proof.
+  intros.
+  (* why we cannot rewrite H? *)
+  (* rewrite H. *)
+  eapply open_safety_inv_ref. reflexivity. eauto. auto.
+Qed.
+
+
+
